add incremental proofs to credit default swap

proofs/oracle_based_loan.v
@@ -1,65 +1,93 @@
 Load metaproperties.
-Definition PayWithPenalty (sum : nat)
-           (penalty_addr : Address) :=
-  (And
-     (Scale sum (One USD))
-     (ScaleObs penalty_addr (One USD))).
 
-Definition PenaltyCtr (sum : nat)
-           (oracle_payment_check penalty_addr : Address) :=
-  (If (oracle_payment_check)
-      Zero
-      (Give (PayWithPenalty sum penalty_addr))).
 
-Definition Oracle_based_loan
-           (sum : nat) (now period : nat)
-           (oracle_salary_check
-              oracle_payment_check
-              penalty_addr : Address) :=
-  If oracle_salary_check
-     (And
-        (Give (Scale sum (One USD)))
-        (Give
-           (After (now + period)
-                  (PenaltyCtr sum oracle_payment_check penalty_addr))))
+(*
+Credit default swap
+
+Assume that Alice holds a financial obligation from
+a company called C whose price is P = 1000 dollars.
+The maturity of the obligation is M = 3 years:
+C pays a fee per year of FY = 100 dollars to Alice,
+and at the end of the 3 years (maturity reached)
+it pays back to Alice P, that is, 1000 dollars.
+Therefore, Alice should receive
+
+  P + M * FY = 1000 + (3 * 100)
+
+dollars at the end of the 3 years.
+
+Since Alice knows that C has financial issues and it is
+possible that C may not be able to pay the yearly fees
+(i.e., C defaults), Alice buys a Credit Swap Derivative
+(CDS) from a bank B.
+A CDS acts as an insurance: Alice pays a fee of F = 20
+dollars per year to B, and in exchange, B will pay
+1000 + (YL * 100) dollars if C. That is, B pays to Alice
+P + YL * 100, where YL is the number of years left until
+the obligation reaches its maturity.
+For instance, if C defaults in the first year, YL = M - 1
+and B pays P + YL * 100 = 1000 + 200 = 1200 dollars to Alice.
+
+Here we want to prove that Alice recovers P + M * FY, that is,
+1300 dollars.
+The bank B receives a fee F = k * 20 from Alice, where
+k = M - YL.
+*)
+
+
+Definition pay_sum (sum : nat) (c : Currency) :=
+  Scale sum (One c).
+
+Definition default_payment (defaulted_addr : Address)
+           (price FY : nat) (YL : Time) :=
+  If defaulted_addr
+     (pay_sum (price + (YL * FY)) USD)
      Zero.
 
-Check query.
-Proposition PayWithPenalty_I_to_O :
-  forall s1 s2 s ctr_id dsc_id I O ctr t sum penalty_addr penalty,
+Definition yearly_check (defaulted_addr : Address)
+           (price FY F : nat) (YL time : Time) :=
+  And (Give (pay_sum F USD))
+      (At time (default_payment defaulted_addr price FY YL)).
+
+Definition CDS (Alice C : Address)
+           (defaulted_addr : Address)
+           (price FY F : nat) (YL now : Time)
+  :=
+  (
+    And
+      (yearly_check defaulted_addr price FY F 3 (now + 1))
+      (
+        And (yearly_check defaulted_addr price FY F 2 (now + 2))
+            (yearly_check defaulted_addr price FY F 1 (now + 3))
+      )
+  ).
+
+(* The issuer pays the owner *)
+Proposition pay_sum_I_to_O :
+  forall s1 s2 ctr_id dsc_id I O ctr t sum c,
     consistent_state s1 ->
-    ctr = finctr ctr_id dsc_id (PayWithPenalty sum penalty_addr) I O O 1 ->
-    joins_in_s O ctr s1 s s2 t ->
+    ctr = finctr ctr_id dsc_id (pay_sum sum c) I O O 1 ->
+    joins O ctr s1 s2 t ->
     O <> 0 ->
-    query (m_gateway s1) penalty_addr t = Some penalty ->
     (exists tr,
       In tr (m_ledger s2) /\
       tr_ctr_id tr = ctr_id /\
       tr_from tr = I /\
       tr_to tr = O /\
-      tr_amount tr = sum)  /\ 
-    exists tr',
-      In tr' (m_ledger s2) /\
-      tr_ctr_id tr' = ctr_id /\
-      tr_from tr' = I /\
-      tr_to tr' = O /\
-      tr_amount tr' = penalty.
+      tr_amount tr = sum).
 Proof.
   intros.
-  destruct_join_in_s H1.
+  destruct_join H1.
   - insert_consistent s Ss.
     induction St; subst s'.
     + inversion_event Ev. find_contradiction Ev.
     + ctr_case_analysis ctr ctr0.
-      execute_own ctr H10. clear H11. subst t.
-      case_match H10; try inversion H10.
-      destruct r. inversion H12. clear H12. subst.
-      case_match H0; try inversion H0. subst.
-      inversion H13. subst. clear H13.
-      split; eexists; split. 
-      * eapply steps_does_not_remove_transactions; eauto.
-        simpl. subst ledger'. left. trivial.
-      repeat split; trivial. resolve_owner H4.
+      execute_own ctr H9. inversion H9. clear H9. subst.
+      simpl in *.
+      eexists. split.
+      * eapply steps_does_not_remove_transactions; eauto; simpl. left. trivial.
+      * repeat split; trivial. resolve_owner H4.
+        simpl. omega.
     + not_or ctr ctr0 H6.
     + not_or ctr ctr0 H6.
     + ctr_case_analysis ctr ctr0. inversion_event Ev. find_contradiction Ev.
@@ -74,80 +102,110 @@ Proof.
     + find_contradiction_del Ev.
 Qed.
 
-
-(* The issuer receives scale * 10 EUR from the owner (who joins) *)
-Proposition frce_I_to_O :
-  forall s1 s2 ctr_id dsc_id I O sc ctr t,
+(* If the payment is defaulted, then the insurance pays the
+ price + YL * FY *)
+Proposition defaulted_payment_true :
+  forall s1 s2 s ctr_id dsc_id I O ctr t response defaulted_addr FY YL price,
     consistent_state s1 ->
-    ctr = finctr ctr_id dsc_id frce_desc I O O sc ->
-    joins O ctr s1 s2 t ->
+    ctr = finctr ctr_id dsc_id (default_payment defaulted_addr price FY YL) I O O 1 ->
+    joins_in_s O ctr s1 s2 s t ->
     O <> 0 ->
-    exists tr,
+    query (m_gateway s) defaulted_addr (m_global_time s) = Some response ->
+    response <> 0 ->
+    (exists tr,
       In tr (m_ledger s2) /\
       tr_ctr_id tr = ctr_id /\
       tr_from tr = I /\
       tr_to tr = O /\
-      tr_amount tr = sc * 10 /\
-      tr_currency tr = EUR.
+      tr_amount tr = price + (YL * FY)).
 Proof.
   intros.
-  destruct_join H1.
+  destruct_joins_in H1.
   - insert_consistent s Ss.
-    induction St; subst s'.
+    induction St; subst s0.
     + inversion_event Ev. find_contradiction Ev.
     + ctr_case_analysis ctr ctr0.
-      execute_own ctr H9.
-      inversion H9.
-      eexists. split.
-      eapply steps_does_not_remove_transactions; eauto.
-      simpl. subst ledger'. simpl. left. trivial.
-      repeat split; trivial. resolve_owner H4.
-    + not_or ctr ctr0 H6.
-    + not_or ctr ctr0 H6.
+      execute_own ctr H11.
+      rewrite H3 in H11.
+      case_eq (response); intros; subst response.
+      * contradiction.
+      *
+        simpl in H11.
+        inversion H11.
+        subst.
+        eexists. split.
+        eapply steps_does_not_remove_transactions; eauto.
+        simpl. left. trivial.
+        repeat split; trivial. resolve_owner H6.
+        simpl. omega.
+    + not_or ctr ctr0 H8.
+    + not_or ctr ctr0 H8.
     + ctr_case_analysis ctr ctr0. inversion_event Ev. find_contradiction Ev.
     + find_contradiction Ev.
   - insert_consistent s Ss.
-    induction St; subst s'.
+    induction St; subst s0.
     + inversion_event Ev. find_contradiction_del Ev.
     + ctr_case_analysis ctr ctr0. inversion_event Ev. find_contradiction_del Ev.
-    + not_or ctr ctr0 H6.
-    + not_or ctr ctr0 H6.
-    + ctr_case_analysis ctr ctr0. execute_own ctr H7. inversion H7.
+    + not_or ctr ctr0 H8.
+    + not_or ctr ctr0 H8.
+    + ctr_case_analysis ctr ctr0. execute_own ctr H9.
+      rewrite H3 in H9.
+      case_eq (response); intros; subst response; simpl in *; try contradiction.
+      inversion H9.
     + find_contradiction_del Ev.
 Qed.
 
-Print frce_I_to_O.
+
+(* Definition yearly_check (defaulted_addr : Address) *)
+(*            (price FY F : nat) (YL time : Time) := *)
+(*   And (Give (pay_sum F USD)) *)
+(*       (At time (default_payment defaulted_addr price FY YL)). *)
 
 
-(* The owner receives scale * 11 USD from the issuer *)
-Proposition frce_O_to_I :
-  forall s1 s2 ctr_id dsc_id I O sc ctr t,
+
+(*
+If the C fails to pay the yearly fee (FY), then
+the bank B should pay Alice price + (YL * FY),
+where YL is the number of years left until maturity.
+Alice should pay upfront an yearly fee F to B.
+ *)
+Proposition yearly_check_default_true_Alice_rights :
+  forall s1 s2 s ctr_id dsc_id I O ctr defaulted_addr price FY F YL time response,
     consistent_state s1 ->
-    ctr = finctr ctr_id dsc_id frce_desc I O O sc ->
-    joins O ctr s1 s2 t ->
+    ctr = finctr ctr_id dsc_id (yearly_check defaulted_addr price FY F YL time) I O O 1 ->
+    joins_in_s O ctr s1 s2 s time ->
     O <> 0 ->
-    exists tr,
+    query (m_gateway s) defaulted_addr (m_global_time s) = Some response ->
+    response <> 0 ->
+    (exists tr,
       In tr (m_ledger s2) /\
       tr_ctr_id tr = ctr_id /\
-      tr_from tr = O /\
-      tr_to tr = I /\
-      tr_amount tr = sc * 11 /\
-      tr_currency tr = USD.
+      tr_from tr = I /\
+      tr_to tr = O /\
+      tr_amount tr = price + (YL * FY)).
 Proof.
   intros.
-  destruct_join H1.
+  destruct_joins_in H1.
   - insert_consistent s Ss.
-    induction St; subst s'.
+    induction St; subst s0.
     + inversion_event Ev. find_contradiction Ev.
     + ctr_case_analysis ctr ctr0.
-      execute_own ctr H9.
-      inversion H9.
-      eexists. split.
-      eapply steps_does_not_remove_transactions; eauto.
-      simpl. subst ledger'. simpl. right. left. trivial.
-      repeat split; trivial. resolve_owner H4.
-    + not_or ctr ctr0 H6.
-    + not_or ctr ctr0 H6.
+      execute_own ctr H11.
+      case_eq (response); intros; subst response; try contradiction.
+      rewrite H3 in H11. simpl in H11.
+      case_match H11.
+      case_if H11.
+      case_if H15.
+      * destruct r. inversion H16. subst.
+        eexists. split.
+        ** inversion H14.
+           eapply steps_does_not_remove_transactions; eauto.
+           simpl. subst ledger'. simpl. left. trivial.
+        ** repeat split; trivial. resolve_owner H6.
+           simpl. omega.
+      * 
+    + not_or ctr ctr0 H8.
+    + not_or ctr ctr0 H8.
     + ctr_case_analysis ctr ctr0. inversion_event Ev. find_contradiction Ev.
     + find_contradiction Ev.
   - insert_consistent s Ss.
